src/Set_Proc.thy
@@ -1,5 +1,5 @@
 theory Set_Proc                
-  imports Set_Calculus Typing Realisation
+  imports Set_Calculus Typing Realisation HF_Extras
 begin
 
 section \<open>Basic Definitions\<close>
@@ -789,7 +789,7 @@ qed
 
 lemma type_term_inf:
   assumes "type_term v1 t = Some l1" "type_term v2 t = Some l2"
-  shows "type_term (v1 \<sqinter> v2) t = Some (l1 \<sqinter> l2)"
+  shows "type_term (inf v1 v2) t = Some (inf l1 l2)"
   using assms
   apply(induction t arbitrary: l1 l2)
        apply(auto simp: type_term.simps inf_min split: if_splits Option.bind_splits)
@@ -798,14 +798,14 @@ lemma type_term_inf:
 lemma types_pset_atom_inf:
   fixes a :: "'a pset_atom"
   assumes "v1 \<turnstile> a" "v2 \<turnstile> a"
-  shows "v1 \<sqinter> v2 \<turnstile> a"
+  shows "inf v1 v2 \<turnstile> a"
   using assms
   by (auto simp: type_term_inf types_pset_atom.simps inf_nat_def)
 
 lemma types_pset_fm_inf:
   fixes \<phi> :: "'a pset_fm"
   assumes "v1 \<turnstile> \<phi>" "v2 \<turnstile> \<phi>"
-  shows "v1 \<sqinter> v2 \<turnstile> \<phi>"
+  shows "inf v1 v2 \<turnstile> \<phi>"
   using assms types_pset_atom_inf
   unfolding types_pset_fm_def by blast
 
@@ -838,14 +838,14 @@ proof -
   with \<open>V \<noteq> {}\<close> have m_x: "\<forall>v \<in> V. m_x x x \<le> v x" "m_x x \<in> V" for x
     using arg_min_nat_le arg_min_natI by (metis ex_in_conv)+
 
-  define M where "M \<equiv> Finite_Set.fold (\<sqinter>) (SOME v. v \<in> V) (m_x ` vars b)"
+  define M where "M \<equiv> Finite_Set.fold inf (SOME v. v \<in> V) (m_x ` vars b)"
   note finite_imageI[where ?h=m_x, OF finite_vars_branch[of b]]
   note M_inf_eq = Inf_fin.eq_fold[symmetric, OF this, of "SOME v. v \<in> V"]
   have M_leq: "M x \<le> v x" if "x \<in> vars b" "v \<in> V" for x v
   proof -
     from that have "m_x x \<in> m_x ` vars b"
       by blast
-    then have "M = m_x x \<sqinter> (\<Sqinter>\<^sub>f\<^sub>i\<^sub>n insert (SOME v. v \<in> V) (m_x ` vars b))"
+    then have "M = inf (m_x x) (\<Sqinter>\<^sub>f\<^sub>i\<^sub>n insert (SOME v. v \<in> V) (m_x ` vars b))"
       unfolding M_def M_inf_eq
       by (simp add: Inf_fin.in_idem finite_vars_branch)
     with m_x that show ?thesis
@@ -860,11 +860,11 @@ proof -
   next
     case (insert x F)
     then have M'_eq: "\<Sqinter>\<^sub>f\<^sub>i\<^sub>n insert (SOME v. v \<in> V) (m_x ` insert x F)
-      = m_x x \<sqinter> (\<Sqinter>\<^sub>f\<^sub>i\<^sub>n insert (SOME v. v \<in> V) (m_x ` F))" (is "_ = ?M'")
+      = inf (m_x x) (\<Sqinter>\<^sub>f\<^sub>i\<^sub>n insert (SOME v. v \<in> V) (m_x ` F))" (is "_ = ?M'")
       by (simp add: insert_commute)
     from types_pset_fm_inf insert have "\<forall>\<phi> \<in> set b. ?M' \<turnstile> \<phi>"
       using V_def m_x(2) by blast
-    moreover have "(w \<sqinter> v) x = 0" if "x \<notin> vars b" "w \<in> V" "v \<in> V" for w v
+    moreover have "(inf w v) x = 0" if "x \<notin> vars b" "w \<in> V" "v \<in> V" for w v
       using that by (simp add: V_def)
     with "insert.IH" m_x(2) have "\<forall>x. x \<notin> vars b \<longrightarrow> ?M' x = 0"
       by (simp add: V_def)
@@ -1094,35 +1094,36 @@ next
   qed
 qed
 
-definition I :: "'a pset_term \<Rightarrow> V" where
+definition I :: "'a pset_term \<Rightarrow> hf" where
   "I \<equiv> SOME f. inj_on f (subterms b)
-             \<and> (\<forall>p. card (elts (f p)) > 2 * card (base_vars b \<union> subterms' b))"
+             \<and> (\<forall>p. hcard (f p) > 2 * card (base_vars b \<union> subterms' b))"
+
 
 lemma (in -) Ex_set_family:
   assumes "finite P"
-  shows "\<exists>I. inj_on I P \<and> (\<forall>p. card (elts (I p)) \<ge> n)"
+  shows "\<exists>I. inj_on I P \<and> (\<forall>p. hcard (I p) \<ge> n)"
 proof -
   from \<open>finite P\<close> obtain ip where ip: "bij_betw ip P {..<card P}"
     using to_nat_on_finite by blast
-  let ?I = "ord_of_nat o ((+) n) o ip"
+  let ?I = "ord_of o ((+) n) o ip"
   from ip have "inj_on ?I P"
     by (auto simp: inj_on_def bij_betw_def)
-  moreover have "card (elts (?I p)) \<ge> n" for p
-    by auto
+  moreover have "hcard (?I p) \<ge> n" for p
+    by simp
   ultimately show ?thesis
     by auto
 qed
 
 lemma
   shows inj_on_I: "inj_on I (subterms b)"
-    and card_I: "card (elts (I p)) > 2 * card (base_vars b \<union> subterms' b)"
+    and card_I: "hcard (I p) > 2 * card (base_vars b \<union> subterms' b)"
 proof -
   have "\<exists>f. inj_on f (subterms b)
-    \<and> (\<forall>p. card (elts (f p)) > 2 * card (base_vars b \<union> subterms' b))"
+    \<and> (\<forall>p. hcard (f p) > 2 * card (base_vars b \<union> subterms' b))"
     using Ex_set_family finite_subterms_branch by (metis less_eq_Suc_le)
   from someI_ex[OF this]
   show "inj_on I (subterms b)"
-       "card (elts (I p)) > 2 * card (base_vars b \<union> subterms' b)"
+       "hcard (I p) > 2 * card (base_vars b \<union> subterms' b)"
     unfolding I_def by blast+
 qed
 
@@ -1135,14 +1136,6 @@ proof -
     using wf_branch_not_Nil[OF wf_branch] by blast+
   with inj_on_I show "inj_on I (base_vars b)" "inj_on I (subterms' b)"
     unfolding inj_on_def by blast+
-qed
-
-lemma finite_elts_I: "finite (elts (I t))"
-proof -
-  from card_I have "card (elts (I t)) \<noteq> 0"
-    by (metis less_zeroE)
-  then show "finite (elts (I t))"
-    by (meson card_eq_0_iff)
 qed
 
 definition "eq \<equiv> symcl ({(s, t). AT (s =\<^sub>s t) \<in> set b}\<^sup>=)"
@@ -1232,13 +1225,11 @@ proof -
 qed
 
 lemma finite_eq_class: "finite (eq `` {x})"
-  using finite_subterms_branch finite_subset eq_class_subs_subterms by blast
+  using eq_class_subs_subterms finite_subterms_branch
+  using finite_subset by fastforce
 
-lemma small_eq_class: "small (eq `` {x})"
-  using finite_eq_class[THEN finite_imp_small] .
-
-lemma small_I_image_eq_class[simp, intro]: "small (I ` (eq `` {x}))"
-  using finite_elts_I finite_eq_class Finite_V by simp
+lemma finite_I_image_eq_class: "finite (I ` eq `` {x})"
+  using finite_eq_class by blast
 
 context
 begin
@@ -1252,17 +1243,17 @@ proof(unfold_locales)
 
   from not_dominated_if_base_vars show "\<And>p t. p \<in> base_vars b \<Longrightarrow> \<not> t \<rightarrow>\<^bsub>bgraph b\<^esub> p" .
 
-  from small_eq_class show "\<And>x. small (eq `` {x})" .
+  from finite_eq_class show "\<And>x. finite (eq `` {x})" .
 qed
 
 lemmas realisation = realisation_axioms
 
 lemma card_realisation:
-  "card (elts (realise t)) \<le> 2 * card (subterms b)"
+  "hcard (realise t) \<le> 2 * card (subterms b)"
 proof(induction t rule: realise.induct)
   case (1 x)
-  then have "card (elts (realise x)) = card (realise ` parents (bgraph b) x \<union> I ` eq_class x)"
-    by simp
+  then have "hcard (realise x) = card (realise ` parents (bgraph b) x \<union> I ` eq_class x)"
+    using hcard_HF Zero_hf_def parents_empty_if_base_vars by force
   also have "\<dots> \<le> card (realise ` parents (bgraph b) x) + card (I ` eq_class x)"
     using card_Un_le by blast
   also have "\<dots> \<le> card (parents (bgraph b) x) + card (eq_class x)"
@@ -1287,8 +1278,8 @@ proof(induction t rule: realise.induct)
   finally show ?case .
 next
   case (2 t)
-  then have "card (elts (realise t)) = card (realise ` parents (bgraph b) t)"
-    by simp
+  then have "hcard (realise t) = card (realise ` parents (bgraph b) t)"
+    using hcard_HF[OF finite_realisation_parents] by simp
   also have "\<dots> \<le> card (parents (bgraph b) t)"
     using card_image_le by blast
   also have "\<dots> \<le> card (subterms b)"
@@ -1305,7 +1296,7 @@ qed
 lemma I_neq_realise: "I x \<noteq> realise y"
 proof -
   note card_realisation[of y]
-  moreover have "card (elts (I x)) > 2 * card (subterms b)"
+  moreover have "hcard (I x) > 2 * card (subterms b)"
     using card_I
     by (simp add: subterms_branch_eq_if_wf_branch wf_branch wits_subterms_eq_base_vars_Un_subterms')
   ultimately show ?thesis
@@ -1340,19 +1331,19 @@ proof -
 qed
 
 lemma realise_pwits:
-  "x \<in> Var ` pwits b \<Longrightarrow> realise x = vset {I x}"
+  "x \<in> Var ` pwits b \<Longrightarrow> realise x = HF {I x}"
   unfolding realise.simps(1)[OF pwits_subs_base_vars[THEN subsetD]]
   by (auto simp: eq_class_singleton_if_pwits parents_empty_if_pwits)
 
 lemma I_in_realise_if_base_vars[simp]:
-  "s \<in> base_vars b \<Longrightarrow> I s \<in> elts (realise s)"
+  "s \<in> base_vars b \<Longrightarrow> I s \<^bold>\<in> realise s"
   using refl_eq by (simp add: refl_on_def)
 
 lemma realise_neq_if_base_vars_and_subterms':
   assumes "s \<in> base_vars b" "t \<in> subterms' b"
   shows "realise s \<noteq> realise t"
 proof -
-  from assms have "I s \<notin> elts (realise t)"
+  from assms have "I s \<^bold>\<notin> realise t"
     using I_neq_realise by auto
   with I_in_realise_if_base_vars assms(1) show ?thesis
     by metis
@@ -1380,7 +1371,7 @@ lemma AF_eq_branch_wits_subtermsD:
 
 lemma realisation_if_AT_mem:
   assumes "AT (s \<in>\<^sub>s t) \<in> set b"
-  shows "realise s \<in> elts (realise t)"
+  shows "realise s \<^bold>\<in> realise t"
 proof -
   from assms have "t \<in> base_vars b \<union> subterms' b"
     using in_subterms'_if_AT_mem_in_branch(2) wf_branch by blast
@@ -1443,8 +1434,8 @@ proof -
     case subterms'
     have "False" if "realise s \<noteq> realise t"
     proof -
-      from that have "elts (realise s) \<noteq> elts (realise t)"
-        by blast
+      from that have "hfset (realise s) \<noteq> hfset (realise t)"
+        by (metis HF_hfset)
       then obtain a s' t' where
         a: "a \<in> realise ` parents (bgraph b) s'"
            "a \<notin> realise ` parents (bgraph b) t'"
@@ -1453,8 +1444,7 @@ proof -
       with subterms' have "s' \<in> subterms' b" "t' \<in> subterms' b"
         by auto
       with a obtain u where u: "a = realise u" "u \<rightarrow>\<^bsub>bgraph b\<^esub> s'"
-        using subterms' dominates_if_mem_realisation small_realisation_parents
-        by auto
+        using subterms' dominates_if_mem_realisation by auto
       then have "u \<noteq> s'"
         using dag_bgraph.adj_not_same by blast
       from u have "AT (u \<in>\<^sub>s s') \<in> set b"
@@ -1462,7 +1452,7 @@ proof -
       note lexpands_eq.intros(1,3)[OF assms(2) this, THEN lexpands.intros(6)]
       with \<open>lin_sat b\<close> s'_t' \<open>u \<noteq> s'\<close> have "AT (u \<in>\<^sub>s t') \<in> set b"
         unfolding lin_sat_def by (auto split: if_splits)
-      from realisation_if_AT_mem[OF this] \<open>a = realise u\<close> have "a \<in> elts (realise t')"
+      from realisation_if_AT_mem[OF this] \<open>a = realise u\<close> have "a \<^bold>\<in> realise t'"
         by blast
       with a show False
         using \<open>t' \<in> subterms' b\<close> by simp
@@ -1480,7 +1470,7 @@ proof(cases "x \<in> base_vars b \<and> y \<in> base_vars b")
   case False
   with assms(3) show ?thesis
     using realise_neq_if_base_vars_and_subterms' I_in_realise_if_base_vars
-    by (metis elts_0 empty_iff realise.elims)
+    by (metis hempty_iff realise.elims)
 next
   case True
   from assms bopen have "x \<noteq> y"
@@ -1509,7 +1499,9 @@ next
     by (metis Image_singleton_iff UNIV_I imageI refl_onD)
 
   with \<open>x \<in> base_vars b \<and> y \<in> base_vars b\<close> show "realise x \<noteq> realise y"
-    by (simp add: parents_empty_if_base_vars)
+    using hunion_hempty_left[unfolded Zero_hf_def]
+    using inj_on_HF[THEN inj_onD] finite_I_image_eq_class
+    by (force simp: parents_empty_if_base_vars)
 qed
 
 lemma Ex_AT_eq_mem_subterms_last_if_subterms':
@@ -1652,7 +1644,7 @@ proof -
       then show ?thesis
       proof cases
         case 1
-        then have "realise s1 \<in> elts (realise t2')"
+        then have "realise s1 \<^bold>\<in> realise t2'"
           using realisation_if_AT_mem
           by (metis "*"(4) t1'_t2'(4) t1'_t2'(5))
         with 1 t1'_t2'(3,4) obtain s2 where
@@ -1674,9 +1666,9 @@ proof -
         with \<open>realise s1 = realise s2\<close> have "(s2, s1) \<in> \<Delta>"
           unfolding \<Delta>_def using \<open>AF (s2 =\<^sub>s s1) \<in> set b\<close> by auto
         moreover
-        have "realise s1 \<in> elts (realise t1')" "realise s2 \<in> elts (realise t1')"
-             "realise s1 \<in> elts (realise t2')" "realise s2 \<in> elts (realise t2')"
-          using \<open>realise s1 \<in> elts (realise t2')\<close> \<open>realise s1 = realise s2\<close>
+        have "realise s1 \<^bold>\<in> realise t1'" "realise s2 \<^bold>\<in> realise t1'"
+             "realise s1 \<^bold>\<in> realise t2'" "realise s2 \<^bold>\<in> realise t2'"
+          using \<open>realise s1 \<^bold>\<in> realise t2'\<close> \<open>realise s1 = realise s2\<close>
           using "*"(4) t1'_t2'(4,5) by auto
         with lemma1_3 have "?h (s2, s1) < ?h (t1', t2')"
           using \<open>s1 \<in> subterms' b\<close> \<open>s2 \<in> subterms' b\<close> t1'_t2'_subterms
@@ -1687,7 +1679,7 @@ proof -
           by (metis (mono_tags, lifting) le_antisym le_eq_less_or_eq nat_neq_iff)
       next
         case 2
-        then have "realise s2 \<in> elts (realise t1')"
+        then have "realise s2 \<^bold>\<in> realise t1'"
           using realisation_if_AT_mem
           by (metis "*"(4) t1'_t2'(4) t1'_t2'(5))
         with 2 t1'_t2'(3,4) obtain s1 where
@@ -1709,9 +1701,9 @@ proof -
         with \<open>realise s1 = realise s2\<close> have "(s1, s2) \<in> \<Delta>"
           unfolding \<Delta>_def using \<open>AF (s1 =\<^sub>s s2) \<in> set b\<close> by auto
         moreover
-        have "realise s1 \<in> elts (realise t1')" "realise s2 \<in> elts (realise t1')"
-             "realise s1 \<in> elts (realise t2')" "realise s2 \<in> elts (realise t2')"
-          using \<open>realise s2 \<in> elts (realise t1')\<close> \<open>realise s1 = realise s2\<close>
+        have "realise s1 \<^bold>\<in> realise t1'" "realise s2 \<^bold>\<in> realise t1'"
+             "realise s1 \<^bold>\<in> realise t2'" "realise s2 \<^bold>\<in> realise t2'"
+          using \<open>realise s2 \<^bold>\<in> realise t1'\<close> \<open>realise s1 = realise s2\<close>
           using "*"(4) t1'_t2'(4,5) by auto
         with lemma1_3 have "?h (s1, s2) < ?h (t1', t2')"
           using \<open>s1 \<in> subterms' b\<close> \<open>s2 \<in> subterms' b\<close> t1'_t2'_subterms
@@ -1730,13 +1722,13 @@ qed
 lemma realisation_if_AF_mem:
   assumes "sat b"
   assumes "AF (s \<in>\<^sub>s t) \<in> set b"
-  shows "realise s \<notin> elts (realise t)"
+  shows "realise s \<^bold>\<notin> realise t"
 proof
-  assume "realise s \<in> elts (realise t)"
+  assume "realise s \<^bold>\<in> realise t"
   from assms have "s \<in> base_vars b \<union> subterms' b"
                   "t \<in> base_vars b \<union> subterms' b"
     using in_subterms'_if_AF_mem_in_branch[OF wf_branch] by blast+
-  from dominates_if_mem_realisation[OF \<open>realise s \<in> elts (realise t)\<close>]
+  from dominates_if_mem_realisation[OF \<open>realise s \<^bold>\<in> realise t\<close>]
   obtain s' where "s' \<rightarrow>\<^bsub>bgraph b\<^esub> t" "realise s = realise s'"
     by blast
   then have "AT (s' \<in>\<^sub>s t) \<in> set b"
@@ -1790,9 +1782,9 @@ proof -
   from assms(2) have "t1 \<squnion>\<^sub>s t2 \<in> subterms' b"
     using base_vars_subs_vars base_vars_Un_subterms'_eq_subterms by blast
 
-  have "elts (realise (t1 \<squnion>\<^sub>s t2)) \<subseteq> elts (realise t1 \<squnion> realise t2)"
+  have "realise (t1 \<squnion>\<^sub>s t2) \<le> realise t1 \<squnion> realise t2"
   proof
-    fix e assume "e \<in> elts (realise (t1 \<squnion>\<^sub>s t2))"
+    fix e assume "e \<^bold>\<in> realise (t1 \<squnion>\<^sub>s t2)"
     then obtain s where s: "e = realise s" "s \<rightarrow>\<^bsub>bgraph b\<^esub> (t1 \<squnion>\<^sub>s t2)"
       using dominates_if_mem_realisation \<open>t1 \<squnion>\<^sub>s t2 \<in> subterms' b\<close>
       by auto
@@ -1801,7 +1793,7 @@ proof -
     with \<open>sat b\<close> consider "AT (s \<in>\<^sub>s t1) \<in> set b" | "AF (s \<in>\<^sub>s t1) \<in> set b"
       unfolding sat_def using bexpands_noparam.intros(3)[OF _ mem_subterms_last, THEN bexpands.intros(1)]
       by blast
-    then show "e \<in> elts (realise t1 \<squnion> realise t2)"
+    then show "e \<^bold>\<in> realise t1 \<squnion> realise t2"
     proof(cases)
       case 1
       with s show ?thesis using realisation_if_AT_mem by auto
@@ -1813,14 +1805,14 @@ proof -
       with s show ?thesis using realisation_if_AT_mem by auto
     qed
   qed
-  moreover have "elts (realise t1 \<squnion> realise t2) \<subseteq> elts (realise (t1 \<squnion>\<^sub>s t2))"
+  moreover have "realise t1 \<squnion> realise t2 \<le> realise (t1 \<squnion>\<^sub>s t2)"
   proof
-    fix e assume "e \<in> elts (realise t1 \<squnion> realise t2)"
+    fix e assume "e \<^bold>\<in> realise t1 \<squnion> realise t2"
     with \<open>t1 \<in> subterms' b\<close> \<open>t2 \<in> subterms' b\<close> consider
       s1 where "e = realise s1" "s1 \<rightarrow>\<^bsub>bgraph b\<^esub> t1" |
       s2 where "e = realise s2" "s2 \<rightarrow>\<^bsub>bgraph b\<^esub> t2"
       using dominates_if_mem_realisation by force
-    then show "e \<in> elts (realise (t1 \<squnion>\<^sub>s t2))"
+    then show "e \<^bold>\<in> realise (t1 \<squnion>\<^sub>s t2)"
     proof(cases)
       case 1
       then have "AT (s1 \<in>\<^sub>s t1) \<in> set b"
@@ -1865,9 +1857,9 @@ proof -
   from assms(2) have "t1 \<sqinter>\<^sub>s t2 \<in> subterms' b"
     using base_vars_subs_vars base_vars_Un_subterms'_eq_subterms by blast
 
-  have "elts (realise (t1 \<sqinter>\<^sub>s t2)) \<subseteq> elts (realise t1 \<sqinter> realise t2)"
+  have "realise (t1 \<sqinter>\<^sub>s t2) \<le> realise t1 \<sqinter> realise t2"
   proof
-    fix e assume "e \<in> elts (realise (t1 \<sqinter>\<^sub>s t2))"
+    fix e assume "e \<^bold>\<in> realise (t1 \<sqinter>\<^sub>s t2)"
     with \<open>t1 \<sqinter>\<^sub>s t2 \<in> subterms' b\<close> obtain s
       where s: "e = realise s" "s \<rightarrow>\<^bsub>bgraph b\<^esub> (t1 \<sqinter>\<^sub>s t2)"
       using dominates_if_mem_realisation by auto
@@ -1876,12 +1868,12 @@ proof -
     with \<open>sat b\<close> lexpands_int.intros(1)[OF this, THEN lexpands.intros(3)]
     have "AT (s \<in>\<^sub>s t1) \<in> set b" "AT (s \<in>\<^sub>s t2) \<in> set b"
       unfolding sat_def using lin_satD by force+
-    from this[THEN realisation_if_AT_mem] s show "e \<in> elts (realise t1 \<sqinter> realise t2)"
+    from this[THEN realisation_if_AT_mem] s show "e \<^bold>\<in> realise t1 \<sqinter> realise t2"
       by auto
   qed
-  moreover have "elts (realise t1 \<sqinter> realise t2) \<subseteq> elts (realise (t1 \<sqinter>\<^sub>s t2))"
+  moreover have "realise t1 \<sqinter> realise t2 \<le> realise (t1 \<sqinter>\<^sub>s t2)"
   proof
-    fix e assume "e \<in> elts (realise t1 \<sqinter> realise t2)"
+    fix e assume "e \<^bold>\<in> realise t1 \<sqinter> realise t2"
     with \<open>t1 \<in> subterms' b\<close> \<open>t2 \<in> subterms' b\<close> obtain s1 s2 where s1_s2:
       "e = realise s1" "s1 \<rightarrow>\<^bsub>bgraph b\<^esub> t1"
       "e = realise s2" "s2 \<rightarrow>\<^bsub>bgraph b\<^esub> t2"
@@ -1906,7 +1898,7 @@ proof -
     ultimately have "AT (s1 \<in>\<^sub>s t1 \<sqinter>\<^sub>s t2) \<in> set b"
       using \<open>sat b\<close> lexpands_int.intros(6)[OF _ _ mem_subterms_last, THEN lexpands.intros(3)]
       unfolding sat_def by (fastforce simp: lin_satD)
-    from realisation_if_AT_mem[OF this] show "e \<in> elts (realise (t1 \<sqinter>\<^sub>s t2))"
+    from realisation_if_AT_mem[OF this] show "e \<^bold>\<in> realise (t1 \<sqinter>\<^sub>s t2)"
       unfolding \<open>e = realise s1\<close>
       by simp
   qed
@@ -1934,9 +1926,9 @@ proof -
   from assms(2) have "s -\<^sub>s t \<in> subterms' b"
     using base_vars_subs_vars base_vars_Un_subterms'_eq_subterms by blast
 
-  have "elts (realise (s -\<^sub>s t)) \<subseteq> elts (realise s - realise t)"
+  have "realise (s -\<^sub>s t) \<le> realise s - realise t"
   proof
-    fix e assume "e \<in> elts (realise (s -\<^sub>s t))"
+    fix e assume "e \<^bold>\<in> realise (s -\<^sub>s t)"
     then obtain u where u: "e = realise u" "u \<rightarrow>\<^bsub>bgraph b\<^esub> (s -\<^sub>s t)"
       using dominates_if_mem_realisation \<open>s -\<^sub>s t \<in> subterms' b\<close> by auto
     then have "AT (u \<in>\<^sub>s s -\<^sub>s t) \<in> set b"
@@ -1944,13 +1936,13 @@ proof -
     with \<open>sat b\<close> lexpands_diff.intros(1)[OF this, THEN lexpands.intros(4)]
     have "AT (u \<in>\<^sub>s s) \<in> set b" "AF (u \<in>\<^sub>s t) \<in> set b"
       unfolding sat_def using lin_satD by force+
-    with u show "e \<in> elts (realise s - realise t)"
+    with u show "e \<^bold>\<in> realise s - realise t"
       using \<open>sat b\<close> realisation_if_AT_mem realisation_if_AF_mem
       by auto
   qed
-  moreover have "elts (realise s - realise t) \<subseteq> elts (realise (s -\<^sub>s t))"
+  moreover have "realise s - realise t \<le> realise (s -\<^sub>s t)"
   proof
-    fix e assume "e \<in> elts (realise s - realise t)"
+    fix e assume "e \<^bold>\<in> realise s - realise t"
     then obtain u where u:
       "e = realise u" "u \<rightarrow>\<^bsub>bgraph b\<^esub> s" "\<not> u \<rightarrow>\<^bsub>bgraph b\<^esub> t"
       using dominates_if_mem_realisation \<open>s \<in> subterms' b\<close> \<open>t \<in> subterms' b\<close> by auto
@@ -1969,7 +1961,7 @@ proof -
     ultimately have "AT (u \<in>\<^sub>s s -\<^sub>s t) \<in> set b"
       using \<open>sat b\<close> lexpands_diff.intros(6)[OF _ _ mem_subterms_last, THEN lexpands.intros(4)]
       unfolding sat_def by (fastforce simp: lin_satD)
-    from realisation_if_AT_mem[OF this] show "e \<in> elts (realise (s -\<^sub>s t))"
+    from realisation_if_AT_mem[OF this] show "e \<^bold>\<in> realise (s -\<^sub>s t)"
       unfolding \<open>e = realise u\<close>
       by simp
   qed
@@ -1979,7 +1971,7 @@ qed
 lemma realisation_Single:
   assumes "sat b"
   assumes "Single t \<in> subterms b"
-  shows "realise (Single t) = vset {realise t}"
+  shows "realise (Single t) = HF {realise t}"
   using assms
 proof -
   from assms have mem_subterms_last: "Single t \<in> subterms (last b)"
@@ -1993,9 +1985,9 @@ proof -
       by (simp add: assms(2) subterms'_def)
   qed
 
-  have "elts (realise (Single t)) \<subseteq> elts (vset {realise t})"
+  have "realise (Single t) \<le> HF {realise t}"
   proof
-    fix e assume "e \<in> elts (realise (Single t))"
+    fix e assume "e \<^bold>\<in> realise (Single t)"
     then obtain s where s: "e = realise s" "s \<rightarrow>\<^bsub>bgraph b\<^esub> Single t"
       using dominates_if_mem_realisation \<open>Single t \<in> subterms' b\<close> by auto
     then have "AT (s \<in>\<^sub>s Single t) \<in> set b"
@@ -2003,20 +1995,20 @@ proof -
     with \<open>sat b\<close> lexpands_single.intros(2)[OF this, THEN lexpands.intros(5)]
     have "AT (s =\<^sub>s t) \<in> set b"
       unfolding sat_def using lin_satD by fastforce
-    with s show "e \<in> elts (vset {realise t})"
+    with s show "e \<^bold>\<in> HF {realise t}"
       using realisation_if_AT_eq \<open>sat b\<close>[unfolded sat_def]
       by auto
   qed
-  moreover have "elts (vset {realise t}) \<subseteq> elts (realise (Single t))"
+  moreover have "HF {realise t} \<le> realise (Single t)"
   proof
-    fix e assume "e \<in> elts (vset {realise t})"
+    fix e assume "e \<^bold>\<in> HF {realise t}"
     then have "e = realise t"
       by simp
     from lexpands_single.intros(1)[OF mem_subterms_last, THEN lexpands.intros(5)] \<open>sat b\<close>
     have "AT (t \<in>\<^sub>s Single t) \<in> set b"
       unfolding sat_def using lin_satD by fastforce
     from realisation_if_AT_mem[OF this] \<open>e = realise t\<close>
-    show "e \<in> elts (realise (Single t))"
+    show "e \<^bold>\<in> realise (Single t)"
       by simp
   qed
   ultimately show ?thesis by blast
@@ -2121,31 +2113,32 @@ section \<open>Soundness of the Calculus\<close>
 
 subsection \<open>Soundness of Closedness\<close>
 
-lemmas wf_trancl_elts_rel = wf_trancl[OF foundation]
+lemmas wf_trancl_hmem_rel = wf_trancl[OF wf_hmem_rel]
 
-lemma trancl_elts_rel_not_refl: "(x, x) \<notin> {(x, y). x \<in> elts y}\<^sup>+"
-  using wf_trancl_elts_rel by auto
+lemma trancl_hmem_rel_not_refl: "(x, x) \<notin> hmem_rel\<^sup>+"
+  using wf_trancl_hmem_rel by simp
 
 lemma mem_trancl_elts_rel_if_member_seq:
   assumes "member_seq s cs t"
   assumes "cs \<noteq> []"
   assumes "\<forall>a \<in> set cs. I\<^sub>s\<^sub>a M a"
-  shows "(I\<^sub>s\<^sub>t M s, I\<^sub>s\<^sub>t M t) \<in> {(x, y). x \<in> elts y}\<^sup>+"
+  shows "(I\<^sub>s\<^sub>t M s, I\<^sub>s\<^sub>t M t) \<in> hmem_rel\<^sup>+"
   using assms
 proof(induction rule: member_seq.induct)
   case (2 s s' u cs t)
   show ?case
   proof(cases cs)
     case Nil
-    with 2 show ?thesis by auto
+    with 2 show ?thesis
+      unfolding hmem_rel_def by auto
   next
     case (Cons c cs')
-    with 2 have "(I\<^sub>s\<^sub>t M u, I\<^sub>s\<^sub>t M t) \<in> {(x, y). x \<in> elts y}\<^sup>+"
+    with 2 have "(I\<^sub>s\<^sub>t M u, I\<^sub>s\<^sub>t M t) \<in> hmem_rel\<^sup>+"
       by simp
     moreover from 2 have "I\<^sub>s\<^sub>a M (s \<in>\<^sub>s u)"
       by simp
     ultimately show ?thesis
-      by (simp add: trancl_into_trancl2)
+      unfolding hmem_rel_def by (simp add: trancl_into_trancl2)
   qed
 qed simp_all
 
@@ -2162,9 +2155,9 @@ proof -
       unfolding Atoms_def by fastforce
     from memberCycle obtain s where "member_seq s cs s"
       using member_cycle.elims(2) by blast
-    with memberCycle \<open>\<forall>a \<in> set cs. I\<^sub>s\<^sub>a M a\<close> have "(I\<^sub>s\<^sub>t M s, I\<^sub>s\<^sub>t M s) \<in> {(x, y). x \<in> elts y}\<^sup>+"
+    with memberCycle \<open>\<forall>a \<in> set cs. I\<^sub>s\<^sub>a M a\<close> have "(I\<^sub>s\<^sub>t M s, I\<^sub>s\<^sub>t M s) \<in> hmem_rel\<^sup>+"
       using mem_trancl_elts_rel_if_member_seq member_cycle.simps(2) by blast  
-    with trancl_elts_rel_not_refl show ?case
+    with trancl_hmem_rel_not_refl show ?case
       by blast
   qed (use interp.simps(4) in \<open>fastforce+\<close>)
   then show ?thesis
@@ -2306,9 +2299,9 @@ proof (induction rule: bexpands_param.induct)
   with this(1)[THEN this(9)] have "I\<^sub>s\<^sub>t M s \<noteq> I\<^sub>s\<^sub>t M t"
     by auto
   then obtain y where y:
-    "y \<in> elts (I\<^sub>s\<^sub>t M s) \<and> y \<notin> elts (I\<^sub>s\<^sub>t M t) \<or>
-     y \<in> elts (I\<^sub>s\<^sub>t M t) \<and> y \<notin> elts (I\<^sub>s\<^sub>t M s)"
-    by (metis V_equalityI)
+    "y \<^bold>\<in> I\<^sub>s\<^sub>t M s \<and> y \<^bold>\<notin> I\<^sub>s\<^sub>t M t \<or>
+     y \<^bold>\<in> I\<^sub>s\<^sub>t M t \<and> y \<^bold>\<notin> I\<^sub>s\<^sub>t M s"
+    by auto
   have "x \<notin> vars s" "x \<notin> vars t"
     using 1 by (auto simp: vars_fm_vars_branchI)
   then have "I\<^sub>s\<^sub>t (M(x := y)) s = I\<^sub>s\<^sub>t M s" "I\<^sub>s\<^sub>t (M(x := y)) t = I\<^sub>s\<^sub>t M t"
